libcrux-ml-dsa/src/specs.rs
@@ -1,40 +1,46 @@
 use hax_lib::*;
 
-#[fstar::replace_body(r#"Seq.length randomness / 3 <= Lib.IntTypes.max_size_t /\
-    Seq.length $randomness / 3 <= Seq.length $out"#)]
-pub(crate) fn rejection_sample_less_than_field_modulus_pre(randomness: &[u8], out: &[i32]) -> Prop {
-    true.into()
-}
+pub mod simd {
+    use super::*;
+    pub mod portable {
+        use super::*;
+        pub mod sample {
+            use super::*;
+            pub fn rejection_sample_less_than_field_modulus_pre(randomness: &[u8], out: &[i32]) -> Prop {
+                (randomness.len() / 3 <= 4_294_967_295 &&
+                randomness.len() / 3 <= out.len()).into()
+            }
 
-#[fstar::replace_body(r#"let s = Spec.MLDSA.Math.rejection_sample_field_modulus $randomness in
-    v $r <= Seq.length out /\ v $r == Seq.length s /\
-    Seq.slice out 0 (v $r) == s"#)]
-pub(crate) fn rejection_sample_less_than_field_modulus_post(randomness: &[u8], out: &[i32], r: usize) -> Prop {
-    true.into()
-}
+            #[fstar::replace_body(r#"let s = Spec.MLDSA.Math.rejection_sample_field_modulus $randomness in
+                v $r <= Seq.length out /\ v $r == Seq.length s /\
+                Seq.slice out 0 (v $r) == s"#)]
+            pub fn rejection_sample_less_than_field_modulus_post(randomness: &[u8], out: &[i32], r: usize) -> Prop {
+                true.into()
+            }
 
-#[fstar::replace_body(r#"Seq.length randomness * 2 <= Lib.IntTypes.max_size_t /\
-    Seq.length $randomness * 2 <= Seq.length $out"#)]
-pub(crate) fn rejection_sample_less_than_eta_equals_2_pre(randomness: &[u8], out: &[i32]) -> Prop {
-    true.into()
-}
+            pub fn rejection_sample_less_than_eta_equals_2_pre(randomness: &[u8], out: &[i32]) -> Prop {
+                (randomness.len() * 2 <= 4_294_967_295 &&
+                randomness.len() * 2 <= out.len()).into()
+            }
 
-#[fstar::replace_body(r#"let s = Spec.MLDSA.Math.rejection_sample_eta_2 $randomness in
-    v $r <= Seq.length out /\ v $r == Seq.length s /\
-    Seq.slice out 0 (v $r) == s"#)]
-pub(crate) fn rejection_sample_less_than_eta_equals_2_post(randomness: &[u8], out: &[i32], r: usize) -> Prop {
-    true.into()
-}
+            #[fstar::replace_body(r#"let s = Spec.MLDSA.Math.rejection_sample_eta_2 $randomness in
+                v $r <= Seq.length out /\ v $r == Seq.length s /\
+                Seq.slice out 0 (v $r) == s"#)]
+            pub fn rejection_sample_less_than_eta_equals_2_post(randomness: &[u8], out: &[i32], r: usize) -> Prop {
+                true.into()
+            }
 
-#[fstar::replace_body(r#"Seq.length randomness * 2 <= Lib.IntTypes.max_size_t /\
-    Seq.length $randomness * 2 <= Seq.length $out"#)]
-pub(crate) fn rejection_sample_less_than_eta_equals_4_pre(randomness: &[u8], out: &[i32]) -> Prop {
-    true.into()
-}
+            pub fn rejection_sample_less_than_eta_equals_4_pre(randomness: &[u8], out: &[i32]) -> Prop {
+                (randomness.len() * 2 <= 4_294_967_295 &&
+                randomness.len() * 2 <= out.len()).into()
+            }
 
-#[fstar::replace_body(r#"let s = Spec.MLDSA.Math.rejection_sample_eta_4 $randomness in
-    v $r <= Seq.length out /\ v $r == Seq.length s /\
-    Seq.slice out 0 (v $r) == s"#)]
-pub(crate) fn rejection_sample_less_than_eta_equals_4_post(randomness: &[u8], out: &[i32], r: usize) -> Prop {
-    true.into()
+            #[fstar::replace_body(r#"let s = Spec.MLDSA.Math.rejection_sample_eta_4 $randomness in
+                v $r <= Seq.length out /\ v $r == Seq.length s /\
+                Seq.slice out 0 (v $r) == s"#)]
+            pub fn rejection_sample_less_than_eta_equals_4_post(randomness: &[u8], out: &[i32], r: usize) -> Prop {
+                true.into()
+            }
+        }
+    }
 }
