libcrux-ml-dsa/proofs/fstar/extraction/Libcrux_ml_dsa.Simd.Portable.Sample.fsti
@@ -5,25 +5,36 @@ open FStar.Mul
 
 val rejection_sample_less_than_field_modulus (randomness: t_Slice u8) (out: t_Slice i32)
     : Prims.Pure (t_Slice i32 & usize)
-      (requires Libcrux_ml_dsa.Specs.rejection_sample_less_than_field_modulus_pre randomness out)
+      (requires
+        Libcrux_ml_dsa.Specs.Simd.Portable.Sample.rejection_sample_less_than_field_modulus_pre randomness
+          out)
       (ensures
         fun temp_0_ ->
           let out_future, r:(t_Slice i32 & usize) = temp_0_ in
-          Libcrux_ml_dsa.Specs.rejection_sample_less_than_field_modulus_post randomness out_future r
-      )
+          Libcrux_ml_dsa.Specs.Simd.Portable.Sample.rejection_sample_less_than_field_modulus_post randomness
+            out_future
+            r)
 
 val rejection_sample_less_than_eta_equals_2_ (randomness: t_Slice u8) (out: t_Slice i32)
     : Prims.Pure (t_Slice i32 & usize)
-      (requires Libcrux_ml_dsa.Specs.rejection_sample_less_than_eta_equals_2_pre randomness out)
+      (requires
+        Libcrux_ml_dsa.Specs.Simd.Portable.Sample.rejection_sample_less_than_eta_equals_2_pre randomness
+          out)
       (ensures
         fun temp_0_ ->
           let out_future, r:(t_Slice i32 & usize) = temp_0_ in
-          Libcrux_ml_dsa.Specs.rejection_sample_less_than_eta_equals_2_post randomness out_future r)
+          Libcrux_ml_dsa.Specs.Simd.Portable.Sample.rejection_sample_less_than_eta_equals_2_post randomness
+            out_future
+            r)
 
 val rejection_sample_less_than_eta_equals_4_ (randomness: t_Slice u8) (out: t_Slice i32)
     : Prims.Pure (t_Slice i32 & usize)
-      (requires Libcrux_ml_dsa.Specs.rejection_sample_less_than_eta_equals_4_pre randomness out)
+      (requires
+        Libcrux_ml_dsa.Specs.Simd.Portable.Sample.rejection_sample_less_than_eta_equals_4_pre randomness
+          out)
       (ensures
         fun temp_0_ ->
           let out_future, r:(t_Slice i32 & usize) = temp_0_ in
-          Libcrux_ml_dsa.Specs.rejection_sample_less_than_eta_equals_4_post randomness out_future r)
+          Libcrux_ml_dsa.Specs.Simd.Portable.Sample.rejection_sample_less_than_eta_equals_4_post randomness
+            out_future
+            r)
